{"metadata":{"language_info":{"name":"python","version":"3.7.8","mimetype":"text/x-python","codemirror_mode":{"name":"ipython","version":3},"pygments_lexer":"ipython3","nbconvert_exporter":"python","file_extension":".py"},"kernelspec":{"name":"python3","display_name":"Python 3","language":"python"}},"nbformat_minor":5,"nbformat":4,"cells":[{"cell_type":"code","source":"# Importing numpy\nfrom numpy import *\n# Defining matrices A and B as arrays\nA = array([[2, 1, 3], [5, 4, 7], [7, 8, 2]],dtype=float)\nB = array([7,11,4],dtype=float)\nn=len(B)\n# solution vector z with zero value as default\nz=zeros(n,float)\n# Fixed rows from 0 to n-1\nfor k in range(n-1):\n  # Rows under the fixed row\n  for i in range(k+1,n):\n    if A[i,k]==0: \n      continue\n    fac=A[k,k]/A[i,k]\n    for j in range(k,n):\n      # Equation defined in eq (1a) in the notes\n      A[i,j]=A[i,j]*fac-A[k,j]\n    # Equation defined in eq (1b) in the notes\n    B[i]=B[k]-B[i]*fac\n# outputs of A and B after elimination step of REF\nprint(A)\nprint(B)\nprint(n)\n\n# Substitution step of REF\nz[n-1]=B[n-1]/A[n-1,n-1]\nfor i in range(n-2,-1,-1):\n  summation=0\n  for j in range(i+1,n-1):\n    summation=summation+A[i,j]*z[j]\n  z[i]=[B[i]-summation]/A[i,i]\n\nprint(z)\n","metadata":{"trusted":true},"execution_count":1,"outputs":[{"name":"stdout","text":"[[ 2.          1.          3.        ]\n [ 0.          0.6        -0.2       ]\n [ 0.          0.         -0.93333333]]\n[ 7.          2.6        -0.13333333]\n3\n[1.33333333 4.33333333 0.14285714]\n","output_type":"stream"}],"id":"eef49326-6d8d-4c39-ae05-fc678585b710"},{"cell_type":"code","source":"","metadata":{},"execution_count":null,"outputs":[],"id":"537ef6c0-feba-47cc-86ef-83caa26cc770"}]}